feat: Advent of code, day 7, solution part 1

Sat/Advent/Day7.lean
@@ -1,11 +1,12 @@
 
 import Sat.Lib.Nat
+import Sat.Lib.Array.Instances
 import Sat.Lib.Equiv
+import Sat.Lib.Fold
 import Sat.Lib.Traversable
 import Sat.Quot
 import Sat.Tactics
 import Sat.Advent.IO
-
 
 -- (lean--version)
 -- ("4" "0" "0-nightly-2021-12-05")
@@ -17,10 +18,55 @@ def dist (i j : Nat) : Nat := max (i - j) (j - i)
 def cost (input : Array Nat) (i : Nat) : Nat :=
 input.foldl (λ acc pos => acc + dist pos i) 0
 
-def posToCount : Array Nat → Array Nat := sorry
+def resize (ar : Array α) (x : α) (i : Nat) : Array α :=
+if i < ar.size
+then ar
+else ar ++ Array.mkArray (i - ar.size + 1) x
 
-def cost' (input : Array Nat) (i : Nat) : Array Nat :=
-scanl (λ acc n => _) 0 (posToCount input)
+theorem lt_size_resize {ar : Array α} {x : α} {i : Nat} :
+  i < (resize ar x i).size := by
+simp [resize]; split
+. assumption
+next h =>
+have h := Nat.le_of_not_gt h
+simp [*]
+
+def modifyResize
+  (ar : Array α) (i : Nat) (f : α → α) (y : α) : Array α :=
+let ar := resize ar y i
+let i : Fin ar.size := ⟨i, lt_size_resize⟩
+ar.set i (f <| ar.get i)
+
+def posToCount (ar : Array Nat) : Array Nat :=
+ar.foldl (λ ar x => modifyResize ar x Nat.succ 0) #[]
+
+def linearCost : Fold Nat Nat :=
+Prod.snd <$> Fold.mk (0, 0)
+  (λ (num, costAccum) n =>
+    (num + n, costAccum + num))
+
+def costUp : Array Nat → Array Nat :=
+linearCost.scanl
+-- scanl (λ n (num, costAccum) => (costAccum + num, (num + n, costAccum + num))) (0, 0)
+
+def costDown : Array Nat → Array Nat :=
+scanr (λ n (num, costAccum) => (costAccum + num, (num + n, costAccum + num)))
+  (0, 0)
+
+def cost' (input : Array Nat) : Array Nat :=
+  let counts := posToCount input
+  let lr := costUp counts
+  let rl := costDown counts
+  Array.zipWith lr rl (.+.)
+
+def minCost (input : Array Nat) : Option (Nat × Nat) :=
+cost' input |>.foldlIdx
+  (λ i x => λ
+    | Option.some ((a, b) : Nat × Nat) =>
+      if x < b then some (i, x)
+      else some (a, b)
+    | Option.none => some (i, x) )
+  none
 
 end day7
 
@@ -42,15 +88,28 @@ def parseInput (input : String) : IO (Array Nat) := do
 Array.mk <| (← input.splitOn "," |>.mapM parseNat)
 
 def inputFileName := "Sat/Advent/Day7_input.txt"
+-- #check elab
+-- #check Lean.PrettyPrinter.ppTerm
+-- #check Lean.MonadQuotation
+-- #print Lean.Syntax
+-- #print Lean.Elab.TermElabM
+-- #print Lean.MacroM
+-- #print Lean.MetaM
+-- #check Lean.Syntax
+
+-- #check Lean.MonadRef
 
 def main : IO Unit := do
--- let ar ← parseInput <| (← IO.FS.lines inputFileName).get! 0
-let ar ← parseInput examples
-IO.println <| cost ar 2
-IO.println <| cost ar 3
-IO.println <| cost ar 4
-IO.println <| cost ar 5
-IO.println <| cost ar 1
+let pos ← parseInput <| (← IO.FS.lines inputFileName).get! 0
+-- let pos ← parseInput examples
+let count ← posToCount pos
+-- IO.println <| pos.size
+-- IO.println <| count
+-- IO.println <| posToCount pos
+IO.println <| dump! minCost pos
+-- IO.println <| dump! costUp count
+-- IO.println <| dump! costDown count
+-- IO.println <| dump! cost' pos
 
 #eval main
 
